theories/Dot/lr/lr_lemma.v
@@ -162,23 +162,21 @@ Section Sec.
   Qed.
 
   Lemma Sub_TVMem_Variant' T1 T2 i j l:
-    Γ ⊨ TLater T1, i <: TLater T2, j + i -∗
+    Γ ⊨ T1, i <: T2, j + i -∗
     Γ ⊨ TVMem l T1, i <: TVMem l T2, j + i.
   Proof.
-    iIntros "#IHT /= !>" (ρ v) "#Hg #HT1". setoid_rewrite laterN_plus.
+    iIntros "#Hsub /= !>" (ρ v) "#Hg #HT1". setoid_rewrite laterN_plus.
     iDestruct "HT1" as (d) "#[Hdl #HT1]".
     iExists d; repeat iSplit => //.
     iDestruct "HT1" as (vmem) "[Heq HvT1]".
     iExists vmem; repeat iSplit => //.
-    iIntros. by iApply "IHT".
+    by iApply "Hsub".
   Qed.
 
   Lemma Sub_TVMem_Variant T1 T2 i l:
-    Γ ⊨ TLater T1, i <: TLater T2, i -∗
+    Γ ⊨ T1, i <: T2, i -∗
     Γ ⊨ TVMem l T1, i <: TVMem l T2, i.
-  Proof.
-    iApply (Sub_TVMem_Variant' _ _ _ 0).
-  Qed.
+  Proof. iApply (Sub_TVMem_Variant' _ _ _ 0). Qed.
 End Sec.
 
 Section swap_based_typing_lemmas.
