theories/Dot/misc/misc_dead.v
@@ -70,26 +70,21 @@ Section path_wp.
 
   Lemma path_wp_cl n p v:
     path_wp p (λ w, ⌜ w = v ⌝) ⊢@{iPropI Σ}
-    ▷^(plength p) ⌜ nclosed p n → nclosed_vl v n ⌝.
+    ⌜ nclosed p n → nclosed_vl v n ⌝.
   Proof.
     elim: p v => /= [w|p IHp l] v.
     - iIntros "!%" (->). exact: fv_pv_inv.
-    - rewrite path_wp_eq -swap_later; setoid_rewrite IHp.
+    - rewrite path_wp_eq; setoid_rewrite IHp.
       iDestruct 1 as (w) "[Hpwp H]".
-      iNext (plength p).
       iDestruct "Hpwp" as %Himpl.
-      iDestruct "H" as (? Hl) "> ->". iIntros "!%" (Hclps).
+      iDestruct "H" as (? Hl) "->". iIntros "!%" (Hclps).
       enough (nclosed (dvl v) n). by eauto with fv.
       eapply nclosed_lookup', Himpl; eauto with fv.
   Qed.
 
   Lemma path_wp_timeless_len φ p:
-    (∀ v, Timeless (φ v)) →
-    path_wp p φ ⊢ ▷^(plength p) False ∨ ∃ v, path_wp p (λ w, ⌜ w = v ⌝) ∧ φ v.
-  Proof.
-    rewrite path_wp_eq. intros Htime. iDestruct 1 as (v) "(Heq & Hv)".
-    iDestruct (timeless_timelessN with "Hv") as "[H | H]"; eauto.
-  Qed.
+    path_wp p φ ⊢ ∃ v, path_wp p (λ w, ⌜ w = v ⌝) ∧ φ v.
+  Proof. by rewrite path_wp_eq. Qed.
 
   Fixpoint path2tm p: tm :=
     match p with
@@ -98,24 +93,20 @@ Section path_wp.
     end.
 
   Lemma path_wp_exec p v :
-    path_wp p (λ w, ⌜ w = v ⌝) ⊢@{iPropI Σ} ▷^(plength p) ⌜ PureExec True (plength p) (path2tm p) (tv v) ⌝.
+    path_wp p (λ w, ⌜ w = v ⌝) ⊢@{iPropI Σ}
+    ⌜ PureExec True (plength p) (path2tm p) (tv v) ⌝.
   Proof.
     iInduction p as [w|] "IHp" forall (v); rewrite /PureExec/=.
     - iIntros (-> _). by iIntros "!%"; constructor.
     - iIntros "#Hp" (_). iDestruct (path_wp_eq with "Hp") as (vp) "{Hp}(Hp&Hs)".
       iSpecialize ("IHp" with "Hp"). iClear "Hp".
-      rewrite -swap_later. iNext (plength p).
-      iDestruct "IHp" as %Hpure. iDestruct "Hs" as (vq Hlook) "> ->".
+      iDestruct "IHp" as %Hpure. iDestruct "Hs" as (vq Hlook) "->".
       iIntros "!%". eapply nsteps_r.
       + by apply (pure_step_nsteps_ctx (fill_item (ProjCtx l))), Hpure.
       + apply nsteps_once_inv, pure_tproj, Hlook.
   Qed.
 
   Lemma path_wp_adequacy p φ :
-    (∀ v, Timeless (φ v)) →
-    path_wp p φ ⊢ ▷^(plength p) False ∨ (∃ v, ⌜ PureExec True (plength p) (path2tm p) (tv v) ⌝ ∧ φ v).
-  Proof.
-    intros Htime. rewrite path_wp_timeless_len; iDestruct 1 as "[$|H]".
-    iApply timeless_timelessN. setoid_rewrite path_wp_exec. iNext. eauto.
-  Qed.
+    path_wp p φ ⊢ (∃ v, ⌜ PureExec True (plength p) (path2tm p) (tv v) ⌝ ∧ φ v).
+  Proof. rewrite path_wp_timeless_len. by setoid_rewrite path_wp_exec. Qed.
 End path_wp.
